Progress in prfprp adaptive

theories/paris/examples/prfprp_adaptive.v
@@ -28,7 +28,7 @@ Section prp_prf.
   (** We will prove the PRF/PRP switching lemma.
       We assume that the adversaries are well-typed. *)
   Variable adv : val.
-  Definition TAdv := ((TInput → TOutput) → TBool)%ty.
+  Definition TAdv := ((TInput → (TUnit+ TOutput)) → TBool)%ty.
   Variable adv_typed : (∅ ⊢ₜ adv : TAdv).
   Definition q_calls := q_calls Input.
   Definition PRF := PRF val_size val_size.
@@ -37,9 +37,32 @@ Section prp_prf.
          if: "b" then PRP #false "adv" #() else PRF #false "adv" #(). *)
 
   Local Opaque INR.
+  Local Opaque seq.
 
   Section proofs.
     Context `{!parisRGS Σ}.
+
+    Lemma refines_list_seq_l E K e A (n m : nat) :
+      (∀ v : val, ⌜is_list (seq n m) v⌝ -∗ REL (fill K (of_val v)) << e @ E : A)
+      -∗ REL (fill K (list_seq #n #m)) << e @ E : A.
+    Proof.
+      iIntros "Hlog".
+      iApply refines_wp_l.
+      by iApply wp_list_seq.
+    Qed.
+
+    Lemma refines_list_seq_r E K e A (n m :nat):
+      (∀ v : val, ⌜is_list (seq n m) v⌝ -∗ REL e << (fill K (of_val v)) @ E : A)
+      -∗ REL e << (fill K (list_seq #n #m)) @ E : A.
+    Proof.
+      iIntros "Hlog".
+      iApply refines_step_r.
+      iIntros.
+      iMod (spec_list_seq with "[$]") as "(%&?&?)".
+      iModIntro.
+      iFrame.
+      iApply ("Hlog" with "[$]").
+    Qed.
 
     (* Can we give a nice *amortized* spec for relating
        [q_calls random_function] and [q_calls random_permutation] ? *)
@@ -47,16 +70,122 @@ Section prp_prf.
     Theorem PRP_PRF (Q : nat) ε :
       (INR (fold_left (Nat.add) (seq 0 Q) 0%nat) / INR (S val_size))%R = ε
       →
-      ↯ ε ⊢ (REL (PRP #false adv #() #Q) << (PRF #false adv #() #Q) : lrel_bool).
+      ↯ ε ⊢ (REL (PRP #false adv ((λ: "_", #()),#()) #Q) << (PRF #false adv ((λ: "_", #()),#()) #Q) : lrel_bool).
     Proof with (rel_pures_l ; rel_pures_r).
       iIntros (<-) "Hε".
       rewrite /PRP/PRF/prp.PRP/prf.PRF...
+      rewrite /random_permutation/random_function...
+      rewrite /random_permutation_state...
+      rel_apply_l refines_init_map_l.
+      iIntros (mapref) "mapref"...
+      rel_apply_r refines_init_map_r.
+      iIntros (mapref') "mapref'"...
+      replace 0%Z with (Z.of_nat 0%nat) by lia.
+      rel_apply_l (refines_list_seq_l _ _ _ _ 0%nat).
+      iIntros (?) "%"...
+      rel_alloc_l unused as "unused"...
+      rewrite /query_prp...
+      rel_bind_l (q_calls _ _).
+      rel_bind_r (q_calls _ _).
+      unshelve iApply (refines_bind with "[-][]").
+      { exact (interp (TInput → (TUnit + TOutput)) []). }
+      2: {
+        iIntros (f f') "Hff'".
+        simpl.
+        unshelve iApply (refines_app with "[] [Hff']").
+        3: rel_values.
+        rel_arrow_val.
+        iIntros (o o') "Hoo'". rel_pures_l ; rel_pures_r.
+        repeat rel_apply refines_app. 3: rel_values.
+        Unshelve.
+        3: exact (interp TBool []).
+        1: { rel_arrow_val. iIntros (??) "#(%_&->&->)". rel_pures_l ; rel_pures_r. rel_values. }
+        replace (lrel_arr
+                   (lrel_arr 
+                      lrel_int (lrel_sum lrel_unit lrel_int))
+                   (interp TBool nil)) with
+          (interp TAdv []) by easy.
+        iApply refines_typed.
+        assumption.
+      }
+
+      rewrite /q_calls /prf_cpa.q_calls /bounded_oracle.q_calls...
+      rel_alloc_l counter as "counter".
+      rel_alloc_r counter' as "counter'"...
+      replace 0%Z with (Z.of_nat 0%nat) by lia.
+      erewrite <-fmap_empty.
+      iApply (refines_na_alloc
+                (∃ (q : nat) (M:gmap nat Z) (l:list nat),
+                    ↯ (fold_left Nat.add (seq q Q) 0%nat / S val_size)
+                    ∗ counter ↦ #q
+                    ∗ counter' ↦ₛ #q
+                    ∗ map_list mapref ((λ b, LitV (LitInt b)) <$> M)
+                    ∗ map_slist mapref' ((λ b, LitV (LitInt b)) <$> M)
+                    ∗ ⌜ (size (dom M) <= q)%nat ⌝
+                    ∗ ⌜ ∀ x, x ∈ elements (dom M) -> (x < S val_size)%nat ⌝
+                    ∗ ⌜NoDup l⌝
+                    ∗ ⌜is_list l v⌝
+                    ∗ ⌜(S val_size - q <=length l)%nat⌝  
+                    ∗ unused ↦ v
+                    ∗ ⌜(forall x:nat, x∈ ((map_img M):gset _) -> x ∈ l -> False)⌝
+                    ∗ ⌜∀ x, x ∈ l -> (x<S val_size)%nat ⌝
+                )%I
+                (nroot.@"cpa")); iFrame.
+      iSplit. 
+      { (* solve obligations to establish invariant *)
+        iPureIntro. simpl.
+        eexists _.
+        repeat split; try done.
+        - by set_unfold.
+        - apply NoDup_seq. 
+        - by rewrite seq_length.
+        - intros ?. rewrite elem_of_seq. lia.         
+      }
+      iIntros "#Hinv".
+      rel_arrow_val.
+      iIntros (??) "(%n&->&->)"...
+      rewrite -bool_decide_and.
+      iApply (refines_na_inv with "[$Hinv]"); first done.
+      iIntros "[>(%q&%M&%l&Hε&Hcounter&Hcounter'&Hml&Hml'&%&%&%&%&%&unused&%&%) Hclose]".
+      rel_load_l; rel_load_r...
+      rewrite -bool_decide_and.
+      case_bool_decide; last first.
+      { (* input is not valid or we exceed query num*)
+        idtac...
+        iApply refines_na_close; iFrame.
+        iSplit; first (iPureIntro; by exists l)...
+        rel_values. repeat iExists _. by iLeft.
+      }
+      idtac...
+      rel_load_l; rel_load_r...
+      rel_store_l; rel_store_r...
+      replace n with (Z.of_nat (Z.to_nat n)) by lia.
+      rel_apply_l (refines_get_l with "[-Hml][$Hml]").
+      iIntros (?) "Hml ->".
+      rel_apply_r (refines_get_r with "[-Hml'][$]").
+      iIntros (?) "Hml' ->".
+      destruct (((λ b : Z, #b) <$> M)!!Z.to_nat n) eqn:Hres...
+      { (* we query something from before*)
+        replace (Z.of_nat q+1)%Z with (Z.of_nat (S q)) by lia.
+        iApply refines_na_close; iFrame.
+        iSplitL.
+        - iModIntro. iExists M, l. iFrame.
+          iSplitL.
+          + admit.
+          + iPureIntro; repeat split; (done||lia).
+        - rewrite lookup_fmap_Some in Hres.
+          destruct Hres as (?&<-&?).
+          rel_values. repeat iExists _. iRight. iPureIntro.
+          simpl.
+          repeat split; by eexists _.
+      }
+      
     Admitted.
 
     Theorem PRF_PRP (Q : nat) ε :
       (INR (fold_left (Nat.add) (seq 0 Q) 0%nat) / INR (S val_size))%R = ε
       →
-      ↯ ε ⊢ (REL (PRF #false adv #() #Q) << (PRP #false adv #() #Q) : lrel_bool).
+      ↯ ε ⊢ (REL (PRF #false adv ((λ: "_", #()),#()) #Q) << (PRP #false adv ((λ: "_", #()),#()) #Q) : lrel_bool).
     Proof with (rel_pures_l ; rel_pures_r).
     Admitted.
 
